src/Spec/CompileLoop.v
@@ -1,0 +1,265 @@
+Require Import ConcurProc.
+Require Import Equiv.
+Require Import Helpers.Helpers.
+Require Import FunctionalExtensionality.
+Require Import Omega.
+Require Import List.
+Require Import Compile.
+
+Import ListNotations.
+
+Global Set Implicit Arguments.
+Global Generalizable All Variables.
+
+
+Section Compiler.
+
+  Variable opLoT : Type -> Type.
+  Variable opMidT : Type -> Type.
+
+  Variable compile_op : forall T, opMidT T -> ((opLoT T) * (T -> bool)).
+
+  Fixpoint compile T (p : proc opMidT T) : proc opLoT T :=
+    match p with
+    | Ret t => Ret t
+    | Op op => Until (snd (compile_op op)) (Op (fst (compile_op op)))
+    | Bind p1 p2 => Bind (compile p1) (fun r => compile (p2 r))
+    | Log v => Log v
+    | Atomic p => Atomic (compile p)
+    | Until c p => Until c (compile p)
+    end.
+
+  Inductive compile_ok : forall T (p1 : proc opLoT T) (p2 : proc opMidT T), Prop :=
+  | CompileOp : forall `(op : opMidT T),
+    compile_ok (Until (snd (compile_op op)) (Op (fst (compile_op op)))) (Op op)
+  | CompileOp1 : forall `(op : opMidT T),
+    compile_ok (until1 (snd (compile_op op)) (Op (fst (compile_op op)))) (Op op)
+  | CompileRet : forall `(x : T),
+    compile_ok (Ret x) (Ret x)
+  | CompileExtraRet : forall `(x : T) `(p1 : T -> proc opLoT TF) p2,
+    compile_ok (p1 x) (p2 x) ->
+    compile_ok (Bind (Ret x) p1) (p2 x)
+  | CompileBind : forall `(p1a : proc opLoT T1) (p2a : proc opMidT T1)
+                         `(p1b : T1 -> proc _ T2) (p2b : T1 -> proc _ T2),
+    compile_ok p1a p2a ->
+    (forall x, compile_ok (p1b x) (p2b x)) ->
+    compile_ok (Bind p1a p1b) (Bind p2a p2b)
+  | CompileUntil : forall `(p1 : proc opLoT T) (p2 : proc opMidT T) (c : T -> bool),
+    compile_ok p1 p2 ->
+    compile_ok (Until c p1) (Until c p2)
+  | CompileLog : forall `(v : T),
+    compile_ok (Log v) (Log v).
+
+  Hint Constructors compile_ok.
+
+  Theorem compile_ok_compile :
+    forall `(p : proc _ T),
+      no_atomics p ->
+      compile_ok (compile p) p.
+  Proof.
+    induction p; simpl; intros; eauto.
+    - inversion H0; clear H0; repeat sigT_eq.
+      eauto.
+    - inversion H; clear H; repeat sigT_eq.
+      eauto.
+    - inversion H.
+  Qed.
+
+  Theorem compile_no_atomics :
+    forall `(p : proc _ T),
+      no_atomics p ->
+      no_atomics (compile p).
+  Proof.
+    induction p; simpl; intros; eauto.
+    - inversion H0; clear H0; repeat sigT_eq. eauto.
+    - inversion H; clear H; repeat sigT_eq. eauto.
+    - inversion H.
+  Qed.
+
+  Fixpoint compile_ts (ts : threads_state) : threads_state :=
+    match ts with
+    | nil => nil
+    | t :: ts' =>
+      match t with
+      | NoProc => NoProc
+      | Proc p => Proc (compile p)
+      end :: compile_ts ts'
+    end.
+
+  Theorem compile_ts_ok :
+    forall ts,
+      no_atomics_ts ts ->
+      proc_match compile_ok (compile_ts ts) ts.
+  Proof.
+    induction ts; intros.
+    - unfold proc_match; simpl; intuition eauto.
+      left.
+      repeat rewrite thread_get_nil; eauto.
+    - apply no_atomics_ts_cons in H; intuition idtac.
+      unfold proc_match in *; cbn; intuition eauto.
+      destruct tid; subst.
+      + repeat rewrite thread_get_0.
+        destruct a.
+        * simpl in *.
+          right.
+          do 3 eexists; intuition eauto.
+          eapply compile_ok_compile; eauto.
+        * left; eauto.
+      + repeat rewrite thread_get_S.
+        eapply H3.
+  Qed.
+
+  Theorem compile_ts_no_atomics :
+    forall ts,
+      no_atomics_ts ts ->
+      no_atomics_ts (compile_ts ts).
+  Proof.
+    induction ts; intros.
+    - constructor.
+    - simpl.
+      apply no_atomics_ts_cons in H; intuition idtac.
+      constructor; [ | assumption ].
+      destruct a; eauto.
+      simpl.
+      eapply compile_no_atomics; eauto.
+  Qed.
+
+
+  Variable State : Type.
+  Variable lo_step : OpSemantics opLoT State.
+  Variable hi_step : OpSemantics opMidT State.
+
+  Definition noop_or_success :=
+    forall `(opM : opMidT T) opL cond tid s r s',
+      (opL, cond) = compile_op opM ->
+      lo_step opL tid s r s' ->
+      cond r = false /\ s = s' \/
+      cond r = true /\ hi_step opM tid s r s'.
+
+  Variable is_noop_or_success : noop_or_success.
+
+
+  Lemma compile_ok_exec_tid : forall T (p1 : proc _ T) p2,
+    compile_ok p1 p2 ->
+    forall tid s s' result evs,
+      exec_tid lo_step tid s p1 s' result evs ->
+      (exists p1',
+        s' = s /\
+        result = inr p1' /\
+        compile_ok p1' p2 /\
+        evs = nil) \/
+      (exists result',
+        exec_tid hi_step tid s p2 s' result' evs /\
+        match result with
+        | inl v => match result' with
+          | inl v' => v = v'
+          | inr _ => False
+          end
+        | inr p' => match result' with
+          | inl v' => p' = Ret v'
+          | inr p'' => compile_ok p' p''
+          end
+        end).
+  Proof.
+    induction 1; intros.
+    - left.
+      exec_tid_inv.
+      eexists; intuition idtac.
+      eauto.
+    - repeat exec_tid_inv.
+      eapply is_noop_or_success in H5.
+      2: rewrite surjective_pairing; eauto.
+      intuition idtac; subst.
+      + left.
+        eexists; intuition idtac.
+        rewrite H0.
+        destruct (Bool.bool_dec false true); try congruence.
+        constructor.
+      + right.
+        eexists; intuition idtac.
+        eauto.
+        simpl.
+        rewrite H0.
+        destruct (Bool.bool_dec true true); try congruence.
+    - right.
+      exec_tid_inv.
+      eexists; intuition idtac.
+      eauto.
+      simpl; eauto.
+    - left.
+      repeat exec_tid_inv.
+      eexists; intuition idtac.
+    - exec_tid_inv.
+      edestruct IHcompile_ok; eauto; intuition idtac.
+      + repeat deex; subst.
+        left.
+        eexists; intuition idtac.
+        eauto.
+      + repeat deex; subst.
+        right.
+        eexists; intuition idtac.
+        eauto.
+        destruct result0; destruct result'; subst; eauto;
+          try solve [ exfalso; eauto ].
+    - right.
+      exec_tid_inv.
+      eexists; intuition idtac.
+      eauto.
+      simpl; eauto.
+      constructor; eauto; intros.
+      destruct (Bool.bool_dec (c x) true); eauto.
+    - right.
+      exec_tid_inv.
+      eexists; intuition idtac.
+      eauto.
+      simpl; eauto.
+  Qed.
+
+  Theorem compile_traces_match_ts :
+    forall ts1 ts2,
+      proc_match compile_ok ts1 ts2 ->
+      traces_match_ts lo_step hi_step ts1 ts2.
+  Proof.
+    unfold traces_match_ts; intros.
+    generalize dependent ts2.
+    destruct H0.
+    induction H; eauto; intros.
+
+    eapply proc_match_pick with (tid := tid) in H2 as H2'.
+    intuition idtac; try congruence.
+    repeat deex.
+    rewrite H in H3; inversion H3; clear H3; subst; repeat sigT_eq.
+
+    edestruct compile_ok_exec_tid; eauto;
+      repeat deex.
+
+    - simpl.
+      eapply IHexec.
+      erewrite <- thread_upd_same with (ts := ts2).
+      eapply proc_match_upd; eauto.
+      eauto.
+
+    - destruct result.
+      + edestruct IHexec.
+          eapply proc_match_del; eauto.
+        eexists; intuition idtac.
+        eapply ExecPrefixOne with (tid := tid).
+          eauto.
+          eauto.
+          destruct result'; eauto; exfalso; eauto.
+        eauto.
+
+      + destruct result'; subst.
+        * 
+
+        * edestruct IHexec.
+            eapply proc_match_upd; eauto.
+          eexists; intuition idtac.
+          eapply ExecPrefixOne with (tid := tid).
+            eauto.
+            eauto.
+            eauto.
+          eauto.
+  Qed.
+
+End Compiler.
